bool/MSetDecide.v
@@ -1,0 +1,4 @@
+Require Import MSets.
+
+Definition var := nat. 
+
