bool/Test.v
@@ -1,5 +1,15 @@
 Require Import Definitions Bool BoolTactic.
 
+Goal forall a b c d e f g,
+  (negb a && b && c && d && e && f && g) ||
+  (a && negb b && c && d && e && f && g) ||
+  (a && b && negb c && d && e && f && g) ||
+  (a && b && c && negb d && e && f && g) ||
+  (a && b && c && d && negb e && f && g) ||
+  (a && b && c && d && e && negb f && g) ||
+  (a && b && c && d && e && f && negb g) = true.
+
+
 Goal forall a b c : bool, c || a = negb (b && negb b && (a || negb a)).
 Proof.
 intros; bool_simpl; unfold var_of_list; simpl.
